generic/Zeta.GenericVerifier.fsti
@@ -1,0 +1,28 @@
+module Zeta.GenericVerifier
+
+open Zeta.Time
+
+(*
+ * Verifier built-in methods
+ *
+ * A verifier thread supports the following built-in methods that can be used
+ * to (a) add records to its internal store (b) evict records from its internal
+ * store; and (c) trigger epoch transitions.
+ *
+ * These are different from application methods that implement application-specific
+ * state machine transitions.
+ *)
+type builtin_method =
+  | AddM                    (* Add a record using Merkle verification *)
+  | EvictM                  (* Evict a record, while protecting it using Merkle *)
+  | AddB                    (* Add a record using Blum verification *)
+  | EvictB                  (* Evict a record using Blum protection *)
+  | EvictBM                 (* Evict a record added using Merkle using Blum protection *)
+  | NextEpoch               (* Transition the verifier thread clock to next epoch *)
+  | VerifyEpoch             (* *)
+
+noeq type verifier_spec =
+  | VSpec: vtls: Type0 ->                             (* type of thread local state *)
+           valid: (vtls -> bool) ->                   (* valid function indicating if the thread is in a valid state *)
+           clock: (v: vtls {valid v} -> timestamp) -> (* for valid states, the clock of the verifier thread *)
+           verifier_spec
