generic/Zeta.Time.fsti
@@ -1,0 +1,58 @@
+module Zeta.Time
+
+(**
+ * Time in zeta is two dimensional, consisting of (epoch, counter). All verifier threads have
+ * internal clocks tracking time of this format and these clocks are used to associate
+ * timestamps to "events" - state machine transitions - which ultimately are used to
+ * characterize correctness.
+ *)
+
+(**
+ * The first component of time in zeta. An epoch is the unit of verification in the sense
+ * all events in an epoch are verified to be correct only after all threads transition
+ * to the next epoch.
+ *)
+let epoch = nat
+
+(**
+ * A counter within an epoch.
+ *)
+let counter = nat
+
+type timestamp =
+  | MkTimestamp: e: epoch ->
+                 c: counter -> timestamp
+
+(* next timestamp *)
+let next (t: timestamp): timestamp =
+  match t with
+  | MkTimestamp e c -> MkTimestamp e (c + 1)
+
+(* return the epoch of a timestamp *)
+let epoch_of (t: timestamp): epoch =
+  match t with
+  | MkTimestamp e _ -> e
+
+(* first timestamp of an epoch *)
+let first (e: epoch): timestamp =
+  MkTimestamp e 0
+
+(* < relation of timestamps *)
+let ts_lt (t1 t2: timestamp) =
+  let e1 = MkTimestamp?.e t1 in
+  let c1 = MkTimestamp?.c t1 in
+  let e2 = MkTimestamp?.e t2 in
+  let c2 = MkTimestamp?.c t2 in
+  e1 < e2 || e1 = e2 && c1 < c2
+
+(* >= relation of timestamps *)
+let ts_geq (t1 t2: timestamp) =
+  not (ts_lt t1 t2)
+
+(* <= relation of timestamps *)
+let ts_leq (t1 t2: timestamp) =
+  t1 = t2 || t1 `ts_lt` t2
+
+(* > relation of timestamps *)
+let ts_gt (t1 t2: timestamp): bool =
+  not (t1 `ts_leq` t2)
